\documentclass[12pt]{article}
\usepackage{fancyhdr}
\usepackage{amsmath}
\usepackage{amssymb, amsmath, graphicx,amsthm,setspace}
\pagestyle{fancy}

\lhead[lh-even]{\textbf{Michael Vu}}  
\lfoot[lf-even]{} 
\chead[ch-even]{\textbf{3.27 Theorem}}  
\cfoot[cf-even]{} 
\rhead[rh-even]{November 4, 2017}  
\rfoot[rf-even]{}

\begin{document}
\noindent\textbf{3.27 Theorem.} Let $a,b,m,n\in\mathbb{Z}$ with $m,n>0$. Then the system

\begin{align*}
x &\equiv a\pmod n\\
x &\equiv b\pmod m
\end{align*}

\noindent has a solution if and only if $(n,m)|(a-b)$.

\bigskip

\noindent\textbf{Proof.} Let the system 

\begin{align*}
x &\equiv a\pmod n\\
x &\equiv b\pmod m
\end{align*}

\noindent have a solution. Since $x\equiv a\pmod n$ and $x\equiv b\pmod m$, \\
$x=a+nt=b+mu$ for $t,u\in\mathbb{Z}$. Thus,

\begin{align*}
nt+a &= mu+b,\\
a-b &= mu - nt.
\end{align*}

\noindent By Theorem 1.48, $(n,m)|(a-b)$. 

\bigskip

\noindent Now let $(n,m)|(a-b)$ be given. By definition, $a-b = (n,m)k$ for $k\in\mathbb{Z}$. By Theorem 1.40, there exists $t',u'\in\mathbb{Z}$ such that $(n,m)=nt'+mu'$. Thus,

\begin{align*}
a-b &= (nt'+mu')k\\
&= nt'k+mu'k,\\
a-nt'k &= b+mu'k.
\end{align*}

\noindent By CPI, let integers $x=a-nt'k=b+mu'k$, $T=-t'k$, and $U=u'k$. We have

\begin{align*}
x &= nT + a & x &= mU + b,\\
x-a &= nT & x - b &= mU.
\end{align*}

\noindent By definition, $x\equiv a\pmod n$ and $x\equiv b\pmod m$. Thus, the system has a solution if and only if $(n,m)|(a-b)$.\qed

\end{document}

