\documentclass[12pt]{article}
\usepackage{fancyhdr}
\usepackage{amsmath}
\usepackage{amssymb, amsmath, graphicx,amsthm,setspace}
\pagestyle{fancy}

\lhead[lh-even]{\textbf{Michael Vu}}  
\lfoot[lf-even]{} 
\chead[ch-even]{\textbf{1.2 Theorem}}  
\cfoot[cf-even]{} 
\rhead[rh-even]{August 30, 2017}  
\rfoot[rf-even]{}

\begin{document}
\noindent\textbf{1.2 Theorem.} Let $a,b,c\in\mathbb{Z}$. If $a\mid b$ and $a\mid c$, then $a\mid (b-c)$.

\bigskip

\noindent\textbf{Proof.} Let $a,b,c\in\mathbb{Z}$ be given such that $a\mid b$ and $a\mid c$. We may choose $k,m\in\mathbb{Z}$ such that $b=ka$ and $c=ma$. Subtracting, we find


\begin{align*}
b-c &= ka- ma \\
&= a(k-m).
\end{align*}


\noindent By CPI, we may choose $f\in\mathbb{Z}$ such that $k-m=f$. Therefore, $b-c=fa$, and by definition, $a\mid(b-c)$.\qed



\end{document}