\documentclass[12pt]{article}
\usepackage{fancyhdr}
\usepackage{amsmath}
\usepackage{amssymb, amsmath, graphicx,amsthm,setspace}
\pagestyle{fancy}

\lhead[lh-even]{\textbf{Michael Vu}}  
\lfoot[lf-even]{} 
\chead[ch-even]{\textbf{A.18 Theorem}}  
\cfoot[cf-even]{} 
\rhead[rh-even]{September 5, 2017}  
\rfoot[rf-even]{}

\begin{document}
\noindent\textbf{A.18 Theorem.} For every natural number $n$, $1+2+2^2+\cdots +2^n= 2^{n+1}-1$.

\bigskip

\noindent\textbf{Proof.} Let $P(n)$ be the statement $1+2+2^2+\cdots +2^n= 2^{n+1}-1$. We consider the base case where $n=0$. 

\bigskip

\noindent For $P(0)$,


\begin{align*}
2^0 &= 2^{0+1}-1, \\
1 &= 2-1 \\
&= 1.
\end{align*}


\noindent Since the base case is true, we will prove by induction. Suppose now, $1+2+2^2+\cdots +2^k= 2^{k+1}-1$ for some natural number $k$. We want to show $1+2+2^2+\cdots +2^k +2^{k+1}= 2^{k+2}-1$. It follows,


\begin{align*}
1+2+2^2+\cdots +2^k+2^{k+1} &= 2^{k+1}-1 +2^{k+1} \\
&= 2(2^{k+1})-1 \\
&= 2^{k+2}-1.
\end{align*}


\noindent Since $P(k+1)$ is true, given $P(k)$ is true, and the base case of $P(n=0)$ is true, $1+2+2^2+\cdots +2^n= 2^{n+1}-1$ is true by induction.\qed

\end{document}