\documentclass[12pt]{article}
\usepackage{fancyhdr}
\usepackage{amsmath}
\usepackage{amssymb, amsmath, graphicx,amsthm,setspace}
\pagestyle{fancy}

\lhead[lh-even]{\textbf{Michael Vu}}  
\lfoot[lf-even]{} 
\chead[ch-even]{\textbf{A.21 Theorem}}  
\cfoot[cf-even]{} 
\rhead[rh-even]{September 5, 2017}  
\rfoot[rf-even]{}

\begin{document}
\noindent\textbf{A.21 Theorem.} For every natural number $n$, $1^3+2^3+3^3+\cdots +n^3 = (1+2+3+\cdots +n)^2$.

\bigskip

\noindent\textbf{Proof.} Let $P(n)$ be the statement $1^3+2^3+3^3+\cdots +n^3 = (1+2+3+\cdots +n)^2$. We consider the base case where $n=1$. 

\bigskip

\noindent For $P(1)$,


\begin{align*}
1^3 &= (1)^2, \\
1 &= 1.
\end{align*}


\noindent Since the base case is true, we will prove by induction. Suppose now, $1^3+2^3+3^3+\cdots +k^3 = (1+2+3+\cdots +k)^2$ for some natural number $k$. We want to show $1^3+2^3+3^3+\cdots +k^3+(k+1)^3 = (1+2+3+\cdots +(k+1))^2$. By Theorem A.10, we know the right side to be $\frac{(k+1)^2(k+2)^2}{4}$. 

\bigskip
\noindent Examining the left side of the equation,


\begin{align*}
1^3+2^3+3^3+\cdots +k^3+(k+1)^3 &= (1+2+3+\cdots +k)^2 + (k+1)^3 \\
&= \left(\frac{k(k+1)}{2}\right)^2+(k+1)^3 \\
&= \frac{k^2(k+1)^2}{4}+(k+1)^3 \\
&= \frac{k^2(k+1)^2+4(k+1)^3}{4} \\
&= \frac{(k+1)^2[k^2+4(k+1)]}{4} \\
&= \frac{(k+1)^2(k^2+4k+4)}{4} \\
&= \frac{(k+1)^2(k+2)^2}{4}.
\end{align*}


\noindent Since $P(k+1)$ is true, given $P(k)$ is true, and the base case of $1^3+2^3+3^3+\cdots +n^3 = (1+2+3+\cdots +n)^2$ for every natural number $n$ is true by induction.\qed

\end{document}